theories/interop/wrappersem.v
@@ -1,0 +1,187 @@
+From stdpp Require Import base strings list gmap.
+From melocoton Require Import multirelations.
+From melocoton.interop Require Import assums basics wrapperstate.
+
+Inductive ml_or_c (A B: Type) : Type :=
+  | ML : A → ml_or_c A B
+  | C : B → ml_or_c A B.
+
+Arguments ML {A B}.
+Arguments C {A B}.
+
+Section wrappersem.
+Context {WPms: WrapperParameters}.
+
+Definition stateW : Type :=
+  (* state of the wrapper, which depends on whether we are yielding control to
+     ML or executing the wrapped C program. *)
+  ml_or_c
+    (wrapstateML * store)
+    (wrapstateC * memory).
+
+Definition func : Type := string.
+
+(* the wrapped C program accepts incoming function calls with ML values as
+   arguments, and produces an ML value as output. *)
+(* we don't have callbacks yet, so there's no "make an external call"
+   expression: the wrapped C program can only be called into, not make "external
+   calls" to ML yet. *)
+Inductive exprW : Type :=
+  | ValW (v : val)
+  | RunningW (ec : exprC)
+  | CallFunctionW (fn : func) (vs : list val).
+
+Definition ectxW : Type := unit.
+Definition fillW : ectxW → exprW → exprW := λ _ e, e.
+
+Definition apply_func (fn : func) (vs : list val) : exprW :=
+  CallFunctionW fn vs.
+
+Definition wrapper_step (prog : progC) : mrel (exprW * stateW) (exprW * stateW) :=
+  λ '(e, ρ) φ,
+    (* step in the underlying wrapped C program *)
+    (∀ ec ρc mem ec' mem',
+       e = RunningW ec →
+       ρ = C (ρc, mem) →
+       head_step_C prog ec mem ec' mem' →
+       φ (RunningW ec', C (ρc, mem')))
+    ∨
+    (* incoming call of a C function from ML *)
+    (∀ fn vs ρml σ,
+       e = CallFunctionW fn vs →
+       ρ = ML (ρml, σ) →
+       ∃ χ ζ privσ lvs,
+         is_store χ ζ privσ σ ∧
+         ML_change_lstore (χML ρml) (ζML ρml) ζ ∧
+         ML_extends_lloc_map (ζML ρml) (χML ρml) χ ∧
+         Forall2 (is_val χ ζ) vs lvs ∧
+         ∀ ws mem ρc,
+           (∀ γ (a:addr) v,
+              (rootsML ρml) !! a = Some v →
+              reachable ζ [v] γ →
+              γ ∈ dom (gset lloc) (θC ρc)) →
+           Forall2 (repr_lval (θC ρc)) lvs ws →
+           repr (θC ρc) (rootsML ρml) (privmemML ρml) mem →
+           χC ρc = χ →
+           ζC ρc = ζ →
+           rootsC ρc = dom (gset addr) (rootsML ρml) →
+           privσC ρc = privσ →
+           φ (RunningW (apply_func_C fn ws), C (ρc, mem)))
+    ∨
+    (* wrapped C function returning to ML *)
+    (∀ ec w ρc mem,
+       e = RunningW ec →
+       to_val_C ec = Some w →
+       ρ = C (ρc, mem) →
+       ∃ σ lv v ρml,
+         freeze_lstore (ζC ρc) (ζML ρml) ∧
+         (χC ρc) ⊆ (χML ρml) ∧
+         is_store (χML ρml) (ζML ρml) (privσC ρc) σ ∧
+         repr_lval (θC ρc) lv w ∧
+         is_val (χML ρml) (ζML ρml) v lv ∧
+         dom (gset addr) (rootsML ρml) = rootsC ρc ∧
+         repr (θC ρc) (rootsML ρml) (privmemML ρml) mem ∧
+         φ (ValW v, ML (ρml, σ)))
+    ∨
+    (* call from C to the "alloc" primitive *)
+    (∀ K ec tgnum tg sz ρc mem,
+       e = RunningW (fillC K ec) →
+       to_call_C ec = Some ("alloc", [tgnum; sz]) →
+       ρ = C (ρc, mem) →
+       tgnum = tag_as_int tg →
+       (0 < sz)%Z →
+       ∃ roots privmem,
+         dom (gset addr) roots = rootsC ρc ∧
+         repr (θC ρc) roots privmem mem ∧
+         ∀ γ a mem' ρc',
+           γ ∉ dom (gset lloc) (ζC ρc) →
+           ζC ρc' = {[ γ := (Mut, tg, List.repeat (Lint 0) (Z.to_nat sz)) ]} ∪ (ζC ρc) →
+           repr (θC ρc') roots privmem mem' →
+           (θC ρc') !! γ = Some a →
+           (∀ a v γ,
+              roots !! a = Some v →
+              reachable (ζC ρc) [v] γ →
+              γ ∈ dom (gset lloc) (θC ρc')) →
+           χC ρc' = χC ρc →
+           rootsC ρc' = rootsC ρc →
+           privσC ρc' = privσC ρc →
+           φ (RunningW (fillC K (of_val_C a)), C (ρc', mem')))
+    ∨
+    (* call to "registerroot" *)
+    (∀ K ec w ρc mem,
+       e = RunningW (fillC K ec) →
+       to_call_C ec = Some ("registerroot", [w]) →
+       ρ = C (ρc, mem) →
+       w ∉ rootsC ρc →
+       ∀ ρc',
+         rootsC ρc' = {[ w ]} ∪ rootsC ρc →
+         χC ρc' = χC ρc →
+         ζC ρc' = ζC ρc →
+         θC ρc' = θC ρc →
+         privσC ρc' = privσC ρc →
+         φ (RunningW (fillC K (of_val_C 0%Z)), C (ρc', mem)))
+    ∨
+    (* call to "unregisterroot" *)
+    (∀ K ec w ρc mem,
+       e = RunningW (fillC K ec) →
+       to_call_C ec = Some ("unregisterroot", [w]) →
+       ρ = C (ρc, mem) →
+       w ∈ rootsC ρc →
+       ∀ ρc',
+         rootsC ρc' = rootsC ρc ∖ {[ w ]} →
+         χC ρc' = χC ρc →
+         ζC ρc' = ζC ρc →
+         θC ρc' = θC ρc →
+         privσC ρc' = privσC ρc →
+         φ (RunningW (fillC K (of_val_C 0%Z)), C (ρc', mem)))
+    ∨
+    (* call to "modify" *)
+    (∀ K ec w i w' ρc mem γ lv blk blk',
+       e = RunningW (fillC K ec) →
+       to_call_C ec = Some ("modify", [w; i; w']) →
+       ρ = C (ρc, mem) →
+       (0 ≤ i)%Z →
+       repr_lval (θC ρc) (Lloc γ) w →
+       (ζC ρc) !! γ = Some blk →
+       repr_lval (θC ρc) lv w' →
+       modify_block blk (Z.to_nat i) lv blk' →
+       ∀ ρc',
+         χC ρc' = χC ρc →
+         ζC ρc' = <[ γ := blk' ]> (ζC ρc) →
+         θC ρc' = θC ρc →
+         rootsC ρc' = rootsC ρc →
+         privσC ρc' = privσC ρc →
+         φ (RunningW (fillC K (of_val_C 0%Z)), C (ρc', mem)))
+    ∨
+    (* call to "readfield" *)
+    (∀ K ec w i ρc mem γ mut tag lvs lv w',
+       e = RunningW (fillC K ec) →
+       to_call_C ec = Some ("readfield", [w; i]) →
+       ρ = C (ρc, mem) →
+       (0 ≤ i)%Z →
+       repr_lval (θC ρc) (Lloc γ) w →
+       (ζC ρc) !! γ = Some (mut, tag, lvs) →
+       lvs !! (Z.to_nat i) = Some lv →
+       repr_lval (θC ρc) lv w' →
+       φ (RunningW (fillC K (of_val_C w')), C (ρc, mem))
+    )
+    ∨
+    (* call to "val2int" *)
+    (∀ K ec ρc mem w w',
+       e = RunningW (fillC K ec) →
+       to_call_C ec = Some ("val2int", [w]) →
+       ρ = C (ρc, mem) →
+       repr_lval (θC ρc) (Lint w') w →
+       φ (RunningW (fillC K (of_val_C w')), (C (ρc, mem)))
+    )
+    ∨
+    (* call to "int2val" *)
+    (∀ K ec ρc mem w w',
+       e = RunningW (fillC K ec) →
+       to_call_C ec = Some ("int2val", [w]) →
+       ρ = C (ρc, mem) →
+       repr_lval (θC ρc) (Lint w) w' →
+       φ (RunningW (fillC K (of_val_C w')), (C (ρc, mem)))
+    ).
+
+End wrappersem.
